\chapter{Higher-Order Fibonacci Sequences and their Golden Ratios}

% TODO: Add reference to Fibonacci numbers in the continued fraction chapter
The simplest periodic continued fraction is $[1; \overline{1}]$.
This fraction evaluates to the golden ratio and its convergents are ratios of
consecutive Fibonacci numbers.
Naturally, we can consider the simplest vectors $x ∈ ℝ^d$ for the generalized
Euclidean algorithm, where the integer part in each iteration is $1$.
Such vectors can be seen as a multi-dimensional generalization of the golden
ratio and Fibonacci numbers.
However, there does not exist a single definitive golden ratio,
Since the algorithm has an additional freedom in the choice of the pivot.
So there are actually multiple different possible definitions.
Some of these are well known, like the supergolden ratio or the plastic ratio,
which are both roots of cubic polynomials.

Since the definition of the golden ratios depends entirely on the choice of our
pivot element $x_ℓ$, we consider only two strategies in this chapter: First
choosing the smallest fractional value $\{x_ℓ\}$ and second choosing the largest
fractional value $\{x_ℓ\}$.
From these two strategies we will then derive a general definition of
higher-order Fibonacci sequences and their golden ratios.

% ==============================================================================
\section{Higher-Order Fibonacci Sequence for the Minimum Strategy}
% ==============================================================================

We have already seen that the worst-case input for the one-dimensional
Euclidean algorithm are the Fibonacci numbers.
Plugging in two Fibonacci numbers always requires at least n steps for the
algorithm.
This leads to the question whether such numbers also exist in higher dimensions
and what their golden ratios look like.

% TODO: There should be a discussion on what it even means to have a Fibonacci number in higher dimensions

First, we have to understand what Fibonacci numbers in higher dimensions would
look like.
Fibonacci numbers have two properties which make them special for the Euclidean algorithm.
The first is that applying one iteration of the Euclidean algorithm on two
consecutive Fibonacci numbers~$(F(n + 1), F(n))$ yields the previous Fibonacci numbers~$(F(n), F(n - 1))$.
So the Euclidean algorithm requires exactly $n$ steps on this input.

The second property is that they are minimal with respect to this.
There are other sequences, which fulfill the first property, but the Fibonacci
numbers are special, in that they fit exactly once inside the next number.
This means that in the Euclidean algorithm there is a multiplicative factor of $1$ at each step (except the last):
\[
  \begin{array}{rcl}
    F(n + 1) & = & 1 · F(n) + F(n - 1),     \\
    F(n)     & = & 1 · F(n - 1) + F(n - 2), \\
             & ⋮ &                          \\
    F(2)     & = & 2 · F(1).
  \end{array}
\]
Other numbers may have higher factors -- for example, the silver ratio has a
factor of $2$ at each step -- but the Fibonacci numbers have the smallest factor.

This property is also reflected in the fractions $a/b$ for a given input $(a, b)$.
At each step (except the last) the fraction always has an integer part of $1$:
\[
  \begin{array}{rcl}
    \frac{F(n + 1)}{F(n)} & = & 1 + \frac{F(n - 1)}{F(n)},     \\
    \frac{F(n)}{F(n - 1)} & = & 1 + \frac{F(n - 2)}{F(n - 1)}, \\
                          & ⋮ &                                \\
    \frac{F(2)}{F(1)}     & = & 2.                              \\
  \end{array}
\]
So, a higher-dimensional Fibonacci number would also need to have a fraction
with integer part $1$ at each step.

% TODO: We should also discuss the thing about idempotence under the choice of the pivot.
% TODO: Should we have a discussion about why we choose this particular linear system.

First, we are indeed talking about just numbers and not vectors.
The Euclidean algorithm takes one-dimensional integers as input, so one would
expect that the generalized algorithm would take Fibonacci vectors as input.
But the numbers of steps that the algorithm requires only depends on the
initial solution vector x.
In fact, the entire execution of the algorithm only depends on this vector.
There are infinitely many possible linear systems which have the same solution
vector x, and hence there would be infinitely many "Fibonacci vectors".
Therefore, we look instead only for the numbers inside the rational vector.

There are many different possibilities for choosing a linear system which has the solution $x$.
We use a simple construction, which
given a rational vector $x = \left(\frac{p₁}{q}, \frac{p₂}{q}, …, \frac{p_d}{q}\right)$,
constructs the linear system $Bx = c$ with
\begin{equation}
  \label{eq:linear-system-construction}
  B =
  \begin{pmatrix}
    q & 0 & ⋯ & 0 \\
    0 & q & ⋯ & 0 \\
    ⋮ & ⋮ & ⋱ & ⋮ \\
    0 & 0 & ⋯ & q \\
  \end{pmatrix},
  \quad
  c =
  \begin{pmatrix}
    p₁ \\
    p₂ \\
    ⋮ \\
    p_d
  \end{pmatrix}.
\end{equation}

% I would like a better explanation of what the goal of this section is

Although we have reduced the problem just to the vector $x$, there is still
some ambiguity left, when extending Fibonacci numbers to higher dimensions.
The generalized Euclidean algorithm allows for an additional degree of freedom
by choosing which column vector $B_ℓ$ we swap our vector $c$ with.
Therefore, there cannot be just one definitive Fibonacci number, there are
different ones depending on the choice of our index $ℓ$.

The first strategy one may think of is to choose the index $ℓ$ with the
smallest fractional value.
After all, this gives us the largest decrease in the determinant over one
iteration.
Locally, this would be the highest decrease we can achieve.
So we begin with this strategy and try to find a generalization of Fibonacci
numbers under this strategy.

% TODO: Actually explain how we derive the Fibonacci numbers for this strategy.
% TODO: Should we have a table for the Fibonacci numbers?
% TODO: What about adding references to their OEIS number?

The Fibonacci numbers for this strategy are defined as
\begin{align*}
  F(0) = F(1) = ⋯ = F(d) = 1, \qquad F(n + 1) = F(n) + F(n - 1) + ⋯ + F(n - d).
\end{align*}
For $d = 2, 3, 4$, they are also called the Tribonacci, Tetranacci and Pentanacci numbers.
In general, they are known as the $d$-bonacci numbers.
For these numbers,
We use the solution vector
\[
  x =
  \left(
    \frac{F(n)}{F(n + 1)},\;
    \frac{F(n) + F(n - 1)}{F(n + 1)},\;
    ⋯,\;
    \frac{F(n) + F(n - 1) + ⋯ + F(n + 1 - d)}{F(n + 1)}\;
  \right)
\]
and we can use the construction from Equation~\ref{eq:linear-system-construction}
for the actual input to the generalized Euclidean algorithm.

The smallest fractional value in this vector is $x₁$, so we pivot with $ℓ = 1$ first.
\begin{align*}
  \{x₁'\}
  & = \left\{\frac{1}{\{x₁\}}\right\}
  = \left\{\frac{F(n + 1)}{F(n)}\right\}
  = \frac{F(n - 1) + ⋯ + F(n - d)}{F(n)}.
\end{align*}
This gives us the value for $x_d$, if we would have started with $F(n)$ instead of $F(n+1)$.
The other values in our input vector $x$ are calculated as follows:
\begin{align*}
  \{xᵢ'\}
  & = \left\{\frac{\{xᵢ\}}{\{x₁\}}\right\} \\
  & = \left\{\frac{F(n) + F(n - 1) + ⋯ + F(n + 1 - i)}{F(n + 1)} · \frac{F(n + 1)}{F(n)}\right\} \\
  & = \frac{F(n - 1) + ⋯ + F(n - d)}{F(n)}.
\end{align*}
So in the next iteration the value $x_i$ has the same value as $x_{i+1}$ if we
would have started with $F(n)$.
Therefore, in the next iteration the smallest fractional value must be $x_2$.
We continue this until we have cycled through all variables.

Another example would be the opposite strategy: Choosing the maximum in each iteration.
In this case, the Fibonacci numbers are defined as
\begin{align*}
  F(0) = \dots = F(d) = 1, \qquad F(n + 1) = F(n) + F(n - d).
\end{align*}

The golden ratios for each definition is the limit of consecutive Fibonacci numbers
\[
  φ = \lim_{n → ∞} \frac{F(n + 1)}{F(n)},
\]
where $F(n)$ can be any of the previously defined Fibonacci numbers.


% ==============================================================================
\section{Higher-Order Fibonacci Sequence for the Maximum Strategy}
% ==============================================================================

% ==============================================================================
\section{Generalized Fibonacci Sequences}
% ==============================================================================

Dividing two consecutive Fibonacci numbers approaches the golden ratio as $n$ increases.
The golden ratio is a solution to the equation $x^2 - x - 1 = 0$.
For higher dimensions, we will encounter similar polynomial equations with higher degree.
The goal of this section is to generalize the relationship between linear
recurrences like the Fibonacci sequence with their respective golden ratio.

Since the algorithm expects $x_i$ between $0$ and $1$, we have to use $1/\phi$ instead of $\phi$.
The value $1/\phi$ is the root of another polynomial $x^2 + x - 1$, which is the reciprocal
of the polynomial $x^2 - x - 1$.

\begin{definition}
  Given a polynomial $p = \sum_{i=0}^n a_i x^n$, its \emph{reciprocal polynomial},
  denoted as $p^*$, is defined as
  \[
    p^*(x) = x^n p(x^{-1}) = a_n + a_{n-1} x + \dots + a_0 x^n.
  \]
\end{definition}

\begin{example}
  The reciprocal of the golden ratio polynomial $x^2 - x - 1$ is
  \begin{align*}
    x^2 + x - 1,
  \end{align*}
  which has a root at $\psi = 1/\phi$.
\end{example}

\begin{lemma}
  Let $p$ be a polynomial. Then, $a$ is a root of $p$ if and only if $a^{-1}$ is a root of $p^*$.
\end{lemma}

\begin{proof}
  Let $a$ be a root of $p$. It follows $p^*(a^{-1}) = a^n p(a) = a^n \cdot 0 = 0$.
  Now let $a^{-1}$ be a root of $p^*$. Then $p^*(a^{-1}) = a^n p(a) = 0$.
  By construction, $a$ cannot be zero and therefore we must have $p(a) = 0$.
\end{proof}

\begin{definition}
  A linear recurrence with coefficients~$a_0, \dots, a_d$ is an equation of the
  following form:
  \[
    F(n + 1) = a_0 F(n - d) + a_1 F(n - d + 1) + \dots + a_{d-1} F(n - 1) + a_d F(n).
  \]
\end{definition}

\begin{definition}
  Given a linear recurrence~$F$ with coefficients~$a_0, \dots, a_d$, its
  \emph{characteristic polynomial} $p_F$ is defined as
  \[
    p_F(x) = x^{d+1} - a_d x^d - a_{d-1} x^{d-1} - \dots - a_1 x - a_0.
  \]
\end{definition}

\begin{example}
  The linear recurrence which has $p_d^*(x)$ as its characteristic polynomial is:
  \begin{align*}
    F(n) = F(n - 1) + (-1)^{d+1} F(n - d) - \sum_{i=2}^{d - 1} (-1)^{i+1} 2 F(n - i).
  \end{align*}
\end{example}

% TODO: Show that this converges! We're still missing the convergence criteria
\begin{lemma}
  Let $F$ be a linear recurrence with coefficients $a_0, \dots, a_d$.
  If its characteristic polynomial has a real positive root $\phi$
  and the sequence $F(n+1)/F(n)$ is converging, then
  \[
    \lim_{n \to \infty} \frac{F(n + 1)}{F(n)} = \phi.
  \]
\end{lemma}

\begin{proof}
  By assumption, the ratios approach some limit $L$. It follows:
  \[
    L
    = \lim_{n \to \infty} \frac{F(n + 1)}{F(n)}
    = \lim_{n \to \infty} a_0 + \sum_{i = 1}^d \frac{a_i F(n - d + i)}{F(n)}
  \]
  Each term in the sum can be rewritten as a product of consecutive terms:
  \[
    \frac{F(n - 1 - d + i)}{F(n - 1)}
    = \frac{F(n - 1 - d + i)}{F(n - d + i)} \frac{F(n - d + i)}{F(n - d + i + 1)} \dots \frac{F(n - 2)}{F(n-1)}.
  \]
  Hence, each term in the sum approaches $L^{-i}$,
  which results in the following polynomial:
  \[
    L = a_0 + \sum_{i = 1}^d a_{d - i} L^{-i},
    \quad \text{or equivalently} \quad
    L^{d+1} = a_0 + a_1 L + \dots + a_d L^d,
  \]
  which directly corresponds to a root of its characteristic polynomial.
\end{proof}

\begin{corollary}
  Under the same conditions, $\lim_{n \to \infty} F(n + i) / F(n) = \phi^i$ for $i > 1$.
\end{corollary}

Given, the linear recurrence $F(n + d + 1) = F(n) + a_1 F(n - 1) + \dots + a_d F(n + d)$,
the value for $x_i^{(n)}$ in the solution $x^{(n)}$ is
\begin{equation}
  \label{eq:general-solution}
  x_i^{(n)} = \frac{F(n - i) + \sum_{k=1}^{i-1} a_{d-k} F(n - k)}{F(n)}.
\end{equation}

\begin{lemma}
  Pivoting with the first element of $x^{(n)}$ using the modified update rule yields the vector
  \[
    x' = (x^{(n-1)}_2, x^{(n-1)}_3, \dots, x^{(n-1)}_d, x^{(n-1)}_1).
  \]
\end{lemma}

\begin{proof}
  For $x_1$, we get
  \[
    \begin{aligned}
      \frac{1}{x_1}
      & = \frac{F(n)}{F(n - 1)} \\
      & = a_d + \frac{F(n - d - 1) + a_1 F(n - d - 2) + \dots + a_{d-1} F(n - 2)}{F(n - 1)} \\
      & = a_d + x^{(n-1)}_d.
    \end{aligned}
  \]
  For the other values, we get
  \begin{align*}
    \frac{x_i}{x_1}
    & = \frac{F(n - i) + \sum_{k=1}^{i-1} a_{d-k} F(n - k)}{F(n)} \frac{F(n)}{F(n - 1)} \\
    & = a_{d-1} + \frac{F(n - i) + \sum_{k=2}^{i-1} a_{d-k} F(n - k)}{F(n-1)} \\
    & = x^{(n-1)}_{i+1} \qedhere
  \end{align*}
\end{proof}

\begin{corollary}
  Running the generalized Euclidean algorithm with $x^{(n)}$ as the solution to
  the linear system $B x = c$ requires $n$ steps, if $x^{(n)}_1$ is the
  smallest element in $x^{(n)}$.
\end{corollary}

Of course, the Euclidean algorithm receives a matrix $B \in \Z^{d \times d}$
and vector $c \in \Z^d$ as its input and not the solution $x$ itself.
However, we can construct a very simple linear system $B^{(n)} x = c^{(n)}$,
where $x^{(n)}$ is the solution, in the following way:
\[
  B^{(n)} =
  \begin{pmatrix}
    F(n) & 0 & \dots & 0 & 0 \\
    0 & F(n) & \dots & 0 & 0 \\
    \vdots & \vdots & \ddots & \vdots & \vdots \\
    0 & 0 & \dots & F(n) & 0 \\
    0 & 0 & \dots & 0 & F(n) \\
  \end{pmatrix},
\]
\[
  c^{(n)} =
  \begin{pmatrix}
    F(n - 1) \\
    F(n - 2) + a_{d-1} F(n - 1) \\
    \vdots \\
    F(n - d + 1) + \sum_{k=1}^{d-2} a_{d-k} F(n - k) \\
    F(n - d) + \sum_{k=1}^{d-1} a_{d-k} F(n - k) \\
  \end{pmatrix}.
\]

\begin{lemma}
  The vector $x^{(n)}$ from Equation~\ref{eq:general-solution} is a solution to the
  linear system $B^{(n)} x = c^{(n)}$.
\end{lemma}

\begin{proof}
  Follows directly from the definition of $x^{(n)}$.
\end{proof}

\iffalse
% ==============================================================================
\section{Pivoting the Same Element}
% ==============================================================================

In one dimension, a solution is bad when the value $x_1$ is close to $1$.
However, in the next iteration $x_1$ would be close to $0$ and therefore
would lead to a greater decrease in the determinant.
An initial guess would be that the solution lies exactly between $0$ and $1$ at $1/2$.
However, this solution is also good as after just one step we have achieved integrality.

The solution is to choose a value $x_1$ such that its value in the first
iteration is the same as its value in the second iteration.
This means we are trying to solve the following equation:
\[
  x_1 = 1/x_1 - 1.
\]
This gives us the polynomial $x^2 + x - 1$ where the root is the inverse of the
golden ratio.

% TODO: Explore other strategies. Can we generalize this to every possible strategy?
In just two dimensions, we already have an additional degree of freedom.
Since the solution $x$ consists of two values, we can choose which index we pivot with.
We will choose the value with the smallest fractional value as this decreases
the determinant the fastest.
We assume w.l.o.g. that our values are sorted in increasing order.
This means we pivot with $x_1$ first.

% TODO: What about just choosing the golden ratio for every x_i?
% TODO: Are odd dimensions easier since the decrease is not worse? We could
% choose two values to be the same, since the ratio for odd dimensions is
% smaller than the previous dimension
Just like in one dimension we want to choose $x_1$ carefully such that the
determinant decreases the same amount in every iteration.
A simple solution would be to fill both values with the golden ratio.
In this case, it does not matter which index we choose as each one decreases
the determinant the same amount.
However, in two dimensions we can make this decrease slightly worse
by choosing different values for $x_1$ and $x_2$ such that we swap the pivot
in each iteration.

Assuming the value for $x_1$ is already chosen where would $x_2$ be placed?
Ideally, it would be close to the right side of $x_1$, because then the new
value $-x_2 / x_1$ would be close to $-1$ and the fractional value would be
close to $1$.
Since the decrease must stay the same in each iteration, this gives us the
following two equations:
\begin{align*}
  x_1 = 2 - x_2 / x_1 \\
  x_2 = 1 / x_1 - 1,\\
\end{align*}
which leads to the following polynomial:
\begin{align*}
  x_1^3 - 2x_1^2 - x_1 + 1 = 0
\end{align*}

Let $\phi_2$ be the root of this polynomial.
If we choose $x_1 = \phi_2$ and $x_2 = 2\phi_2 - \phi_2^2$,
then the values in the second iteration are
\[\begin{aligned}
  x_1' & = 1 / x_1 - 1   &  & = 1 / \phi_2 - 1                    &  & = 2\phi_2 + \phi_2^2 &  & = x_2, \\
  x_2' & = 2 - x_2 / x_1 &  & = 2 - (2\phi_2 + \phi_2^2) / \phi_2 &  & = \phi_2             &  & = x_1
\end{aligned}\]

We can extend this to $d$ dimensions using the following equations:
\begin{align*}
  x_1 = 2 - x_2 / x_1 \\
  x_2 = 2 - x_3 / x_1 \\
  x_3 = 2 - x_4 / x_1 \\
  \vdots \\
  x_{d-1} = 2 - x_d / x_1 \\
  x_d = 1 / x_1 - 1 \\
\end{align*}

These leads us to two polynomials depending on the dimension.
\begin{itemize}
  \item For even $d$: $x - 1 + 2 x^2 - 2 x^3 + \dots + x^{d+1}$
  \item For odd $d$: $1 - x - 2 x^2 + 2 x^3 - 2 x^4 \dots + x^{d+1}$
\end{itemize}
or in one equation $p_d(x) := 1 - x - (-x)^{d+1} - \sum_{i = 2}^{d} 2 (-x)^{i} = 0$.
Let $\phi_d$ be the root of this polynomial.
Then, we choose as our solution $x = (x_1, \dots, x_d)$ with
\begin{equation}
  \label{eq:rotate-solution}
  x_1 = \phi_d, \quad x_i = 2 - x_1 x_{i-1} = -(-\phi_d)^i + \sum_{k=0}^{i-1} 2 (-\phi_d)^i.
\end{equation}

\begin{example}
  For $d = 5$, we get the following values:

  \begin{tikzpicture}[scale=10]
    \draw (0.5820216424559055, -0.01) -- node[above] {$x_1$} (0.5820216424559055, 0.01);
    \draw (0.7181491667223714, -0.01) -- node[above] {$x_2$} (0.7181491667223714, 0.01);
    \draw (0.7661126076135922, -0.01) -- node[above] {$x_3$} (0.7661126076135922, 0.01);
    \draw (0.6837042616132034, -0.01) -- node[above] {$x_4$} (0.6837042616132034, 0.01);
    \draw (0.8252940926247403, -0.01) -- node[above] {$x_5$} (0.8252940926247403, 0.01);
    \draw[->] (0, 0) -- (1, 0);
  \end{tikzpicture}
\end{example}

\begin{itemize}
  \item \textbf{Polynomial}:
    \[
      1 - x - (-x)^{d+1} - \sum_{i = 2}^{d} 2 (-x)^{i} = 0.
    \]
  \item \textbf{Algebraic Solution Vector}:
    \[
      x_i = 2x + (-x)^{i+1} + \sum_{k=2}^{i} (-x)^{k}.
    \]
  \item \textbf{Linear Recurrence}:
    \[
      F(n) = F(n - 1) + (-1)^{d+1} F(n - d) - \sum_{i=2}^{d - 1} (-1)^{i+1} 2 F(n - i).
    \]
  \item \textbf{Rational Solution Vector}:
    \[
      x_1 = \frac{F(n - 1)}{F(n)}, x_i = \frac{2 F(n-1) + (-1)^{i+1} F(n - i) + \sum_{k=2}^i (-1)^k F(n-k)}{F(n)}.
    \]
  \item \textbf{Matrix}:
    \[\left(\begin{array}{cccc|c}
      F(n)   & 0      & \dots  & 0      & F(n - 1) \\
        0    & F(n)   & \dots  & 0      & 2 F(n - 1) - F(n - 2) \\
      \vdots & \vdots & \ddots & \vdots & \vdots   \\
        0    & 0      & \dots  & F(n)   & 2 F(n-1) + (-1)^{d+1} F(n - d) + \sum_{k=2}^d (-1)^k F(n-k) \\
    \end{array}\right)\]
\end{itemize}

\begin{example}
  \begin{align*}
    \left\{ \frac{1}{x_1} \right\}
    & = \left\{ \frac{F(n - 1) + 2 F(n - 2) - 2 F(n - 3) + F(n - 4)}{F(n - 1)} \right\} \\
    & = \frac{2 F(n - 2) - 2 F(n - 3) + F(n - 4)}{F(n - 1)} \\
    \left\{ -\frac{x_2}{x_1} \right\}
    & = \left\{ -\frac{2 F(n - 1) - F(n - 2)}{F(n)} \frac{F(n)}{F(n - 1)} \right\} \\
    & = \frac{F(n - 2)}{F(n - 1)} \\
    \left\{ -\frac{x_3}{x_1} \right\}
    & = \left\{ -\frac{2 F(n - 1) - 2 F(n - 2) + F(n - 3)}{F(n)} \frac{F(n)}{F(n - 1)} \right\} \\
    & = \frac{2 F(n - 2) - F(n - 3)}{F(n - 1)}
  \end{align*}
\end{example}
\fi

% ==============================================================================
\section{An Idempotent Solution for Two Dimensions}
% ==============================================================================

Let $\vec x = (\psi, 1 - \psi)$, where $\psi$ is the only real positive root of $x^2 + x - 1$.
For this solution, it does not matter which element we choose to pivot with, it will always
yield the same result.

Pivoting with $x_1$:
\begin{align*}
  \frac{1}{x_1} - 1 & = \frac{1}{\psi} - 1 = \psi, \\
  1 - \frac{x_2}{x_1} & = 1 - \frac{1 - \psi}{\psi} = 1 - \psi.
\end{align*}

Pivoting with $x_2$:
\begin{align*}
  \frac{1}{x_2} - 2 & = \frac{1}{1 - \psi} - 2 = \psi, \\
  1 - \frac{x_1}{x_2} & = 1 - \frac{\psi}{1 - \psi} = 1 - \psi.
\end{align*}

\begin{align*}
  \left(
  \begin{array}{cc|c}
    F(n) & 0    & F(n-1) \\
    0    & F(n) & F(n) - F(n-1) \\
  \end{array}
  \right)
\end{align*}
